riscv_model/code/mul32_lemmas.dfy
@@ -1,0 +1,47 @@
+include "../spec/rsa_ops.dfy"
+
+module mul32_lemmas {
+  
+    import opened bv_ops
+    import opened rv_ops
+    import opened rsa_ops
+    import opened rv_consts
+    import opened powers
+    import opened congruences
+
+    const B  : int := BASE_32;
+    const B2 : int := B * B;
+  
+    lemma mula32_correct_lemma(
+        a: uint32, // x10
+        b: uint32, // x11
+        c: uint32, // x12
+
+        p0: uint32, // ab lower
+        p1: uint32, // ab upper
+
+        p2: uint32, // ab + c lower
+        p3: uint32,
+        p4: uint32, // ab + c upper
+
+        r0: uint64, // ab
+        r1: uint64  // ab + c
+        )
+        
+        requires
+        && p0 == uint32_mul(a, b)
+        && p1 == uint32_mulhu(a, b)
+
+        && p2 == uint32_add(p0, c)
+        && p3 == uint32_lt(p2, p0)
+        && p4 == uint32_add(p1, p3) 
+        
+        && r0 == a * b
+        && r1 == r0 + c
+        ensures
+            to_nat([p2, p4]) == a * b + c;
+    {
+      assert r1 == a *  b + c;
+    }
+
+}
